\include{head}
%\usepackage{maple2e}  ...if needed, disable epsfig in head
%  The following switch distinguishes between homework (solu=0) and its
%  solution (solu=1).
\usepackage{dcolumn}
% \usepackage{stmaryrd}
\newcommand{\bst}{binary search tree\xspace}
\setlength{\leftmargin}{0.00in}
\setlength{\leftmargini}{0.00in}
\setlength{\leftmarginii}{0.00in}
\newcommand{\hwno}{6}
\newcommand{\solu}{1}
\ifthenelse{\equal{\solu}{1}}%
{\renewenvironment{comment}{\  \\ {\bf Solution:\ \ } }}{}%

\begin{document}
\pagestyle{myheadings}
%\newcommand{\pfd}{partial fraction decomposition\xspace}
\ifthenelse{\equal{\solu}{0}}%
{\markboth{{\sc cs504:}{\it \ \ Homework \hwno}}{{\it \ \ Homework \hwno}}}%
{\markboth{{\sc cs504:}{\it \ \ Homework \hwno:  Solutions }}{{\it \ \ %
Homework \hwno:  Solutions}}}

\thispagestyle{empty}
\vspace*{-1.3in}
\begin{center}
\Large{CS504: Analysis of Computations and Systems --- Spring \the\year}
\end{center}

%\voffset=-0.7in
%\hoffset=-0.5in
%\null\vskip 1.1cm
\begin{center}
\ifthenelse{\equal{\solu}{0}}%
{{\large\bf Homework \hwno }\\[1.5ex]}
{{\bf\large \hspace*{0.30in}Solution for Homework \hwno}
\hspace*{0.70in}Posted: \currenttime,\  \today\\[1.5ex]}
\end{center}
\ifthenelse{\equal{\solu}{0}}%
{\hfill Due: Beginning of class, Wednesday, February 26, 2014\\}{}
%
%\begin{center}
%(I shall complete it within a few days)
%\end{center}

% \vspace*{-0.3in}

\begin{enumerate}
\item
In the following $f()$ and $g()$ are the \gf{s} of some
sequences, and therefore have power series developments. The symbols
$z$ and $a$ there are an indeterminate and a constant, respectively.
Explain the relations:\\
$\DS g(z)=f(z-a) ~~~\lar~~(1)~[(z+a)^n]\,f(z)=g_n;
\quad (2)~~ [ z^n ]\,f(z) = \sum_{k} \,\binom{k}{ n} g_k \,a^{k-n} $.\\
This can be used to connect the developments of the same function in two
points.
\begin{comment}
Evidently, if $g(z)=f(z-a)$ holds, presumably for any value of $z$,
then also $g(z+a)=f(z)$.  The \lhs has the expansion
$g(z+a)=\suml_{k\ge0}g_k(z+a)^k$.  Hence the first claim:
$\DS[(z+a)^n]g(z+a) =[(z+a)^n]\suml_{k\ge0}g_k(z+a)^k=g_n$.
And since $g(z+a)=f(z)$, the claim holds.

The second one is more direct:
\[
[z^n]f(z) = [z^n]g(z+a)
=[z^n]\suml_{k\ge0}g_k(z+a)^k
=\suml_{k\ge0}g_k[z^n] \sum_j \binom kj z^ja^{k-j}
=\suml_{k\ge0}g_k \binom kn a^{k-n}
\]
where the extraction operator annihilates all the terms with powers of $z$
which are not $n$.

{\em Now that I am done grading, two comments:}\\
1.  Note the ``annihilation'' or selection action of the operator
$[z^n]$.  It is often useful in simplifying complex expressions, as it
removes one summation level, by selecting a single term out of the summed
over sequence.\\
2.  A note of different kind; a couple of students did more or less what I
write above, but for the binomial expansion used the dummy index $n$ (in
lieu of my $j$), not
noticing that it is already in use, in the extraction operator.
This produced a meaningless mess.  Dummy indices must be ``fresh,'' and
newly-minted. 
\end{comment}
\item
Expand the \ogf $d(x) = (4-2x+x^2)^{-1}$.  Provide for $d_n$ a closed form
expression, without complex numbers.
\begin{comment}
%\mbf{(b)\ \ }
Complex numbers enter the calculation here since the given quadratic does
not have real roots; instead, they are $1\pm i\sqrt3$.  We find
\begin{align*}
d_n &= [x^n]\,\frac1{4-2x+x^2} = [x^n]\frac1{(1-i\sqrt{3} -x)(1+i\sqrt{3}
-x)} =[x^n] \frac i{2\sqrt3}\lp \frac1{1+i\sqrt{3} -x} -\frac1{1-i\sqrt{3}
-x}\rp,
\end{align*}
following a \pfd.  This can be further developed,
\begin{align*}
d_n &= \frac i{2\sqrt3} [x^n] \lp
\frac1{1+i\sqrt3} \frac1{1 -\frac x{1+i\sqrt{3}}}
- \frac1{1-i\sqrt3} \frac1{1 -\frac x{1-i\sqrt{3}}} \rp\\
 &= \frac i{2\sqrt3} \lp
\frac1{1+i\sqrt3} \lp\frac1{1+i\sqrt3} \rp^n
-\frac1{1-i\sqrt3} \lp\frac1{1-i\sqrt3} \rp^n \rp.
\end{align*}
While this involves complex numbers, they are complex conjugates, and the
result of the subtraction is real. The expression can be somewhat
simplified; however, you were asked for an
explicitly real expression, not just real-valued, so we need to continue
beyond a simplification.\\
Since $(1-i\sqrt3) (1+i\sqrt3)=4$, we can write 
$\DS\frac1{1-i\sqrt3} = \frac14\,(1+i\sqrt3)$, and
\[
d_n = \frac i{2\sqrt3}\frac1{4^{n+1}}\lp (1-i\sqrt3)^{n+1}-
(1+i\sqrt3)^{n+1}\rp.
\]
We continue with the polar representation of the complex numbers:
$u+iv=r\,\exp\lp i\tan^{-1} (v/u)\rp$, where $r$ is the absolute value of
the number, $\sqrt{u^2+v^2}$, which is 2 for the numbers we have, and the
tangent of the angle, $\theta$ in the diagram is $\sqrt3$, hence
$\theta=\pi/3$.

\psset{unit=2.2mm,arrows=-,arrowsize=4pt,nodesep=0pt,linewidth=0.6pt}
\begin{pspicture}(-20,-20)(15,20)
% \pscircle[linecolor=blue](25,0){20}
\psline[arrows=->](0,0)(12,0)
\psline[arrows=->](0,-19)(0,19)
\pnode(0,0){orig} \cnode*(10,17.32){1pt}{b} \cnode*(10,-17.32){1pt}{c}
\ncline{orig}{b}\naput[nrot=:U]{$r=2$}
\ncline{orig}{c} \ncline{b}{c}
\rput(14.0, 0){$\Re$}
\rput(-2.0, 17){$\Im$}
\rput(2.6,2.0){$\theta$}
\rput(13.5,17.1){$1+i\sqrt3$}
\rput(13.5,-17.1){$1-i\sqrt3$}
\end{pspicture}

Therefore $1\pm i\sqrt3 = 2e^{\pm i\theta}$, and
$(1\pm i\sqrt3)^{n+1} = 2^{n+1}e^{\pm i(n+1)\pi/3}$.  We use de Moivre
formula, the facts that $\cos(-x)= \cos(x)$ while  $\sin (-x) = -\sin (x)$,
and substitute into $d_n$
\[
d_n = \frac i{2\sqrt3}\frac{2^{n+1}}{4^{n+1}}
\lp \cos (n+1)\frac\pi3 -i \sin (n+1)\frac\pi3 -\cos (n+1)\frac\pi3
-i\sin (n+1)\frac\pi3\rp
\]
The cosines cancel, the sines add, multiplying $i$ by itself corrects the
sign, hence,
\[
d_n= \frac1{2^{n+1}\,\sqrt3}\sin  (n+1)\frac\pi3,
\qquad \text{ while}\quad 
 \sin k\frac\pi3 = \begin{cases} 0& k=3r\\ 
 \frac{\sqrt3}2 & k=6r+1, \quad\text{ or } 6r+2\\
 -\frac{\sqrt3}2 & k=6r-1, \quad\text{ or } 6r-2,\end{cases}
\]
for any integer $r$. Therefore 
\[
d_n=\frac{V_n}{2^{n+2}}, \qquad \text{ where }\quad 
V_n = \begin{cases} 0, & n=3r-1\\ 1, & n=6r, \quad\text{ or }~6r+1\\
 -1,  & n=6r-2, \quad\text{ or }~6r-3. \end{cases}
\]
And then it is always a smart idea to check, and the easiest way is to ask
a computer with an algebra package (I use \map) to do it.  Here it is on
\map, enough to convince me I made no error:
\begin{verbatim}
t := 1/(4-2*x+x^2): series(t, x=0, 12);
1   1     1   3   1   4    1   6    1   7    1    9    1    10   / 12\
- + - x - -- x  - -- x  + --- x  + --- x  - ---- x  - ---- x   +O\x  /
4   8     32      64      256      512      2048      4096  
\end{verbatim}

\end{comment}
\end{enumerate}
\end{document}
\item \label{item4}
\begin{comment}
\end{comment}


\end{enumerate}
\end{document}
\item
\begin{comment}
\end{comment}
\begin{align*}
\end{align*}
\bigskip
\item
\begin{comment}
\end{comment}

\noindent
{\bf Part II.}

Do the following exercises from Heck: {\em Introduction to Maple},
pp63--4:\\
2,\ \ \ 
3(a),(d)\ \ \ 
6,\ \ \ 
11,\ \ \ 
14\\
\noindent
{\bf 3.}
%\rule{6in}{1mm}
\end{document}
