\documentclass[11pt]{article}
\usepackage{times,mathptmx}
\usepackage{amsmath,amsthm,amssymb}
\usepackage{xspace}
\title{CS504 HW9}
\author{Chao Li}
\begin{document}
\maketitle
\section*{2}
\subsection*{a}
\[
\binom{n}{s-t}=\frac{n^{\underline{s-t}}}{(s-t)!}
\]
\[
\binom{n+t}{s}=\frac{(n+t)^{\underline{s}}}{s!}
\]
\begin{align*}
\binom{n}{s-t}&=\binom{n+t}{s}\frac{s(s-1)(s-2)\cdots (s-t+1)}{(n+t)(n+t-1)\cdots (n+t-t+1)} \\
              &=\binom{n+t}{s}\frac{(s-t)^t}{n^t}\underbrace{\cfrac{(1+\cfrac{1}{s-t})(1+\cfrac{2}{s-t})\cdots (1+\cfrac{t}{s-t})}{(1+\cfrac{1}{n})(1+\cfrac{2}{n})\cdots (1+\cfrac{t}{n})}}_{D} \\
\end{align*}
Then partially solve the above equation 
\begin{align*}
D&=\cfrac{1+\cfrac{t(t+1)}{2(s-t)}+\cfrac{t(t+1)(3t^2-13t-2)}{24(s-t)^2}}{1+\cfrac{t(t+1)}{2n}+\cfrac{t(t+1)(3t^2-13t-2)}{24n^2}} \\
 &=\left(1+\frac{t(t+1)}{s(s-t)}\right)\left(1+\frac{t(t+1)}{2n}\right)+o\left(\frac{t^2}{s^2}\right) \\
 &=1+\frac{t(t+1)}{2n}+\frac{t(t+1)}{2(s-t)}+o\left(t^2\left(\frac{1}{n}+\frac{1}{s-t}\right)\right)
\end{align*}
Finally
\[
\binom{n}{s-t}=\binom{n+t}{s}\left(\frac{s-t}{n}\right)^t\cdot D
\]
\subsection*{b}
When \(s=\frac{n}{2}\), then
\[
D=
\]
\end{document}